

# BRAID VARIETIES (V)

2026/01/??

## 1. DIFFERENTIAL FORMS ON $G$

The materials are from [1, Section 3,5] [2, Section 3] and [3, Section 9].

We will embed  $G \hookrightarrow GL_n$ . In the computation below, most of computation reduces to the case  $GL_n$ . We are working over the ring

$$\Omega_G = \mathbb{C}[x_{ij}]_{\text{loc}} \langle dx_{ij} \rangle$$

which is the algebra over  $\mathbb{C}[x_{ij}]_{\text{loc}}$  generated by anti-commutative variables  $dx_{ij}$ . Sometimes we write  $\wedge$  to emphasize that we are working with a non-commutative ring. Let

$$X = \begin{bmatrix} x_{11} & \cdots & x_{1n} \\ \vdots & \ddots & \vdots \\ x_{n1} & \cdots & x_{nn} \end{bmatrix}$$

be a generic element of  $GL_n$ .

Let us consider the **matrix-valued 1-form on  $G$**

$$\theta_L(X) = X^{-1} \cdot dX \in M_n(\Omega_G^1), \quad \theta_R(X) = dX \cdot X^{-1} \in M_n(\Omega_G^1).$$

The forms are left-invariant and right-invariant respectively. That is, if we change variable  $X \mapsto AX$ , then

$$\theta_L(X) = X^{-1}dX \mapsto \theta_L(AX) = (AX)^{-1}d(AX) = X^{-1}A^{-1}AdX = X^{-1}dX = \theta_L(X).$$

Define a **bi-invariant 3-form on  $G$**  by

$$\Omega(X) = \frac{1}{3} \text{Tr}(\theta_L(X)^3) = \frac{1}{3} \text{Tr}(\theta_R(X)^3) \in \Omega_G^3.$$

Note:  $\text{Tr}(AB) = (-1)^{|A||B|} \text{Tr}(BA)$  where  $|A|, |B|$  are the differential degrees. One might prefer the following more Lie-theoretic form of  $\Omega$ :

$$\Omega = \frac{1}{6} \kappa([\theta_L, \theta_L], \theta_L), \quad \kappa(-, -) = \text{Tr}(- \cdot -).$$

Note that after base change to the ring of differential forms, the usual Lie bracket  $[\cdot, \cdot]$  becomes the super commutator, i.e.  $[A, B] = AB - (-1)^{|A||B|}BA$ .

Define a **2-form on  $G \times G$**

$$(X|Y) = \text{Tr}(\theta_L(X)\theta_R(Y)) \in \Omega_{G \times G}^2$$

where  $X \times Y$  is a generic element in  $G \times G$ . We can check the following relations

$$\begin{aligned} d(X, Y) &= \Omega(X) + \Omega(Y) - \Omega(XY) \\ 0 &= (Y, Z) - (XY, Z) + (X, YZ) - (X, Y) \quad (\text{cocycle condition}). \end{aligned}$$

Let me briefly explain the motivation of defining these differential forms.

- It is well-known that the Lie algebra of  $G$  can be identified with the space of right-invariant vector fields. In our case  $G = GL_n$ , the entry of  $dX \cdot X^{-1}$  forms a dual basis of the standard basis of  $\mathfrak{gl}_n$ . Similar for left-invariant vector fields, but the geometric and algebraic brackets differ by a sign.
- One can prove the space of bi-invariant  $k$ -forms over  $G$  coincides with the de Rham cohomology  $H_{dR}^k(G; \mathbb{C})$ . When  $G$  is simple,

$$\dim H_{dR}^k(G; \mathbb{C}) = 1, 0, 0, 1, \dots \quad k = 0, 1, 2, 3, \dots$$

The form  $\Omega$  is the canonical generator of  $H_{dR}^3(G; \mathbb{C})$ .

- As a generator of minimal degree, it is easy to see the cohomology class  $[\Omega]$  is primitive,

$$\text{mult}^*[\Omega] = [\Omega] \otimes 1 + 1 \otimes [\Omega], \text{ i.e. } [\Omega(XY)] = [\Omega(X)] + [\Omega(Y)].$$

However, this is not true before taking cohomology class. The difference is a differential of a 2-form over  $G \times G$ . The 2-form  $(X|Y)$  is one of the choice.

- Associativity of  $\text{mult}$  implies

$$[\Omega(XYZ)] = [\Omega(X)] + [\Omega(Y)] + [\Omega(Z)].$$

There are two ways of proving it via  $d((Y, Z) - (X, YZ))$  and  $d((X, Y) - (XY, Z))$ . They are the same before taking differential  $d$ .

**Example.** When  $G = \mathbb{C}^\times$ .

$$\theta_R(z) = \theta_L(x) = \frac{dx}{x} = d \log(x), \quad \Omega(x) = 0, \quad (x|y) = \frac{dx \wedge dy}{xy} = d \log(x) \wedge d \log(y).$$

**Example.** Assume  $G = GL_2$ . The right-invariant form

$$\begin{aligned} \theta_R(X) &= dX \cdot X^{-1} = \begin{bmatrix} dx_{11} & dx_{12} \\ dx_{21} & dx_{22} \end{bmatrix} \begin{bmatrix} x_{11} & x_{12} \\ x_{21} & x_{22} \end{bmatrix}^{-1} \\ &= \frac{1}{x_{11}x_{22} - x_{12}x_{21}} \begin{bmatrix} dx_{11} & dx_{12} \\ dx_{21} & dx_{22} \end{bmatrix} \begin{bmatrix} x_{22} & -x_{12} \\ -x_{21} & x_{11} \end{bmatrix} \\ &= \frac{1}{x_{11}x_{22} - x_{12}x_{21}} \begin{bmatrix} x_{22}dx_{11} - x_{21}dx_{12} & -x_{12}dx_{11} + x_{11}dx_{12} \\ x_{22}dx_{21} - x_{21}dx_{22} & -x_{12}dx_{21} + x_{11}dx_{22} \end{bmatrix}. \end{aligned}$$

The 3-form  $\Omega(X)$  is given by

$$\frac{1}{(x_{11}x_{22} - x_{12}x_{21})^2} \left( \begin{aligned} &x_{22}dx_{11} \wedge dx_{12} \wedge dx_{21} - x_{21}dx_{11} \wedge dx_{12} \wedge dx_{22} \\ &+ x_{12}dx_{11} \wedge dx_{21} \wedge dx_{22} - x_{11}dx_{12} \wedge dx_{21} \wedge dx_{22} \end{aligned} \right).$$

The 2-form  $(X|Y)$  is

$$\frac{1}{(x_{11}x_{12} - x_{12}x_{21})(y_{11}y_{12} - y_{12}y_{21})} \begin{pmatrix} (x_{21}y_{12} + x_{22}y_{22}) dx_{11} \wedge dy_{11} \\ - (x_{11}y_{12} + x_{12}y_{22}) dx_{21} \wedge dy_{11} \\ - (x_{21}y_{11} + x_{22}y_{21}) dx_{11} \wedge dy_{12} \\ + (x_{11}y_{11} + x_{12}y_{21}) dx_{21} \wedge dy_{12} \\ + (x_{21}y_{12} + x_{22}y_{22}) dx_{12} \wedge dy_{21} \\ - (x_{11}y_{12} + x_{12}y_{22}) dx_{22} \wedge dy_{21} \\ - (x_{21}y_{11} + x_{22}y_{21}) dx_{12} \wedge dy_{22} \\ + (x_{11}y_{11} + x_{12}y_{21}) dx_{22} \wedge dy_{22} \end{pmatrix}.$$

A **twisted symplectic variety** is pair  $(f, \omega)$  where

$$\text{a smooth } M \xrightarrow{f} G \text{ and } \omega \in \Omega_M^2 \text{ such that } d\omega = -f^*\Omega.$$

The most important construction is, we can construct product. We define  $(f_1, \omega_1) \times (f_2, \omega_2) = (f, \omega)$  by

$$f : M_1 \times M_2 \rightarrow G \times G \xrightarrow{\text{mult}} G, \quad \omega = \omega_1 + \omega_2 + (f_1|f_2).$$

This is well-defined since

$$d\omega = d\omega_1 + d\omega_2 + d(f_1|f_2) = -\Omega(f_1) - \Omega(f_2) + (\Omega(f_1) + \Omega(f_2) - \Omega(f_1f_2)).$$

The cocycle condition implies the associativity

$$((f_1, \omega_1) \times (f_2, \omega_2)) \times (f_3, \omega_3) = (f_1, \omega_1) \times ((f_2, \omega_2) \times (f_3, \omega_3)).$$

To describe the product of more factors we introduce a 2-form over  $G^{\times \ell}$

$$(X_1|X_2|\dots|X_\ell) \quad \text{with} \quad (\dots|X|Y|\dots) = (\dots|XY|\dots) + (X|Y).$$

This is well-defined by cocycle condition. Assume  $(f_1, \omega_1) \times \dots \times (f_\ell, \omega_\ell) = (f, \omega)$ , we have

$$f : M_1 \times \dots \times M_\ell \rightarrow G \times \dots \times G \xrightarrow{\text{mult}} G, \\ \omega = \omega_1 + \dots + \omega_\ell + (f_1|\dots|f_\ell).$$

**Example.** When  $G = \mathbb{C}^\times$ . It is easy to compute

$$(x_1|\dots|x_n) = \sum_{1 \leq i < j \leq n} \frac{dx_i dx_j}{x_i x_j}.$$

## 2. DIFFERENTIAL FORMS OVER BRAID VARIETIES

**2.1. A 2-form.** Recall

$$X(\beta) = \{(z_k) : B_{i_1}(z_1) \cdots B_{i_\ell}(z_\ell) \in uB\}, \quad u = \text{Demazure product of } \beta.$$

We define a 2-form over  $X(\beta, u)$  by

$$\omega = (B_{i_1}(z_1)|\dots|B_{i_\ell}(z_\ell)).$$

Note that there are relations between  $z_1, \dots, z_\ell$ .

**Example.** Consider  $G = SL_2$ . Note that

$$\theta_L(B_1(z)) = \begin{bmatrix} 0 & \\ -dz & 0 \end{bmatrix}, \quad \theta_R(B_1(z)) = \begin{bmatrix} 0 & dz \\ & 0 \end{bmatrix}.$$

For  $\beta = \sigma_1^2$ , we have

$$\omega = \text{Trace} \left( \begin{bmatrix} 0 & \\ -dz_1 & 0 \end{bmatrix} \begin{bmatrix} 0 & dz_2 \\ & 0 \end{bmatrix} \right) = -dz_1 \wedge dz_2 = 0.$$

The last equality follows from the relation  $z_1 z_2 = 1$ .

For  $\beta = \sigma_1^3$ , we have

$$\omega = -dz_1 \wedge dz_2 + (-z_2^2)dz_1 \wedge dz_3 - dz_2 \wedge dz_3 = 2 \frac{dz_2 \wedge dz_3}{z_2 z_3 - 1}.$$

The last relation follows from  $z_1 z_2 z_3 = z_1 + z_3$ . Obvious that

$$\omega = 2 \frac{dz_2 \wedge d(z_2 z_3 - 1)}{z_2(z_2 z_3 - 1)} = -2 \frac{dz_3 \wedge d(z_2 z_3 - 1)}{z_3(z_2 z_3 - 1)}.$$

Note that  $z_2, z_3, \boxed{z_2 z_3 - 1}$  are cluster variables.

**Theorem.** For any Demazure weave  $\mathfrak{W} : \beta \rightarrow \sigma_{w_0}$ , using the  $\{\mathbf{A}_v\}$ -variable,

$$\omega \in \text{span}_{\mathbb{Z}} \left( \frac{d\mathbf{A}_{v_1} d\mathbf{A}_{v_2}}{\mathbf{A}_{v_1} \mathbf{A}_{v_2}} \right).$$

Note that the coefficients are functions in  $\{\mathbf{A}_v\}$  a prior .

*Proof.* Let us consider the weave variety  $X(\mathfrak{W}^-)$ . For each region walk from the leftmost region to the rightmost region, we can define a 2-form, by substituting  $B_i(\tilde{z}_e, u_e)$  of  $\tilde{\mathbf{U}}$  in the  $(\cdots | \cdots | \cdots)$ .

- (1) We need to show the 2-form on the bottom walk satisfying the condition;
- (2) We need to show when cross a vertex, the difference satisfying the condition.

Notice that

$$u, u' \text{ are Laurent polynomials in } \{\mathbf{A}_v\} \implies \frac{dud u'}{uu'} \in \text{span}_{\mathbb{Z}} \left( \frac{d\mathbf{A}_{v_1} d\mathbf{A}_{v_2}}{\mathbf{A}_{v_1} \mathbf{A}_{v_2}} \right).$$

The claim (2) follows from direct computation (see Appendix). Let us prove claim (1). On the bottom walk, the 2-form looks like

$$(B_{i_1}(0, u_1) | \cdots | B_{i_l}(0, u_l) | \tilde{\mathbf{U}}_1 | \tilde{\mathbf{U}}_2 | \cdots).$$

Note that  $B_i(0, u) = B_i(0) \chi_i(u)$ . Since  $B_i(0) = \dot{s}_i$  is a constant, we have

$$\begin{aligned} (\cdots | \dot{s}_i | \cdots) &= (\cdots \dot{s}_i | \cdots) = (\cdots | \dot{s}_i \cdots) \\ (\dot{s}_i | X | \cdots) &= (\dot{s}_i X | \cdots) = (X | \cdots). \end{aligned}$$

So we have

$$(\cdots | u^\gamma | \dot{s}_i | \cdots) = (\cdots | u^\gamma \dot{s}_i | \cdots) = (\cdots | \dot{s}_i u^{s_i \gamma} | \cdots) = (\cdots | \dot{s}_i | u^{s_i \gamma} | \cdots).$$

Then we can equivalently written it as

$$(u_1^{\gamma_1} \mid \cdots \mid u_l^{\gamma_l} \mid \tilde{U}_1 \mid \tilde{U}_2 \mid \cdots) = (u_1^{\gamma_1} \mid \cdots \mid u_l^{\gamma_l}) + (u_1^{\gamma_1} \cdots u_l^{\gamma_l} \mid \tilde{U}_1 \mid \tilde{U}_2 \mid \cdots).$$

Note that

$$(u_1^{\gamma_1} \mid \cdots \mid u_l^{\gamma_l}) \in \text{span}_{\mathbb{Z}} \left( \frac{dA_{v_1} dA_{v_2}}{A_{v_1} A_{v_2}} \right)$$

by the computation for  $G = \mathbb{C}^\times$ . Note that

$$X \in B, Y \in \text{Rad}(B) \implies (X|Y) = 0 \quad (\text{since the diagonal entries of } dY \text{ vanish}).$$

The second term vanishes.  $\square$

**2.2. Quivers.** Let us construct an **ice quiver**. The vertices are trivalent vertices  $\mathfrak{W}_3$ . The frozen vertices are those  $v \in \mathfrak{W}_3$  appearing in some bottom  $u$ -labeling. We define the quiver

$$\#\{v_1 \rightarrow v_2\} \text{ or } -\#\{v_1 \leftarrow v_2\} = \text{coefficient of } \frac{dA_{v_1} dA_{v_2}}{A_{v_1} A_{v_2}} \text{ in } \frac{1}{2}\omega.$$

where at least one of  $v_1, v_2$  is unfrozen. We will see the number of arrows is an integer. From the proof, there is a combinatorial description of the coefficients of  $\omega$  and thus the quiver. It has three types of contributions

- the bottom boundary;
- the trivalent vertex;
- the hexavalent vertex.

For an unfrozen vertex  $v_1$  and an arbitrary vertex  $v_2$ , the bottom boundary has no contribution. Let us abbreviate  $A_{v_1} = A_1$  and  $A_{v_2} = A_2$ . Note that

$$\begin{aligned} u &= A_1^{a_1} A_2^{a_2} \cdots \\ u' &= A_1^{a'_1} A_2^{a'_2} \cdots \implies \frac{du du'}{uu'} = \begin{vmatrix} a_1 & a_2 \\ a'_1 & a'_2 \end{vmatrix} \frac{dA_1 dA_2}{A_1 A_2} + \cdots \end{aligned}$$

Then the contribution of trivalent vertices and hexavalent vertices (called **intersection number**)

$$\begin{aligned} & \begin{array}{c} a_1, a_2 \quad b_1, b_2 \\ \diagdown \quad \diagup \\ \text{Y} \\ \diagup \\ c_1, c_2 \end{array} \begin{vmatrix} 1 & 1 & 1 \\ a_1 & c_1 & b_1 \\ a_2 & c_2 & b_2 \end{vmatrix}, \quad \begin{array}{c} a_1, a_2 \quad b_1, b_2 \quad c_1, c_2 \\ \diagdown \quad \diagup \quad \diagup \\ \text{X} \\ \diagup \quad \diagdown \quad \diagdown \\ p_1, p_2 \quad q_1, q_2 \quad r_1, r_2 \end{array} \begin{vmatrix} 1 & 1 & 1 \\ a_1 & b_1 & c_1 \\ a_2 & b_2 & c_2 \end{vmatrix} - \frac{1}{2} \begin{vmatrix} 1 & 1 & 1 \\ p_1 & q_1 & r_1 \\ p_2 & q_2 & r_2 \end{vmatrix}. \end{aligned}$$

In the above diagram, the labeling is the exponents of  $A_1$  and  $A_2$ . Note that  $p_i + q_i = b_i + c_i$  and  $q_i + r_i = a_i + b_i$ , we have

$$\begin{vmatrix} 1 & 1 & 1 \\ a_1 & b_1 & c_1 \\ a_2 & b_2 & c_2 \end{vmatrix} = \begin{vmatrix} 1 & 2 & 2 \\ a_1 & a_1 + b_1 & b_1 + c_1 \\ a_1 & a_2 + b_2 & b_2 + c_2 \end{vmatrix} \equiv \begin{vmatrix} q_1 + r_1 & p_1 + q_1 \\ q_2 + r_2 & p_2 + q_2 \end{vmatrix} \pmod{2},$$

$$\begin{vmatrix} 1 & 1 & 1 \\ p_1 & q_1 & r_1 \\ p_2 & q_2 & r_2 \end{vmatrix} = \begin{vmatrix} 1 & 1 & 1 \\ p_1 & p_1 + q_1 & q_1 + r_1 \\ p_2 & p_2 + q_2 & q_2 + r_2 \end{vmatrix} \equiv \begin{vmatrix} p_1 + q_1 & q_1 + r_1 \\ p_2 + q_2 & q_2 + r_2 \end{vmatrix} \pmod{2}.$$

The description of quiver is equivalent to the pure combinatorial description in [3, Section 4.4, 4.5, 4.6].

## REFERENCES

- [1] Anton Mellit. Toric stratifications of character varieties *Publications mathématiques de l'IHÉS* [arXiv:1905.10685](#). (old name: Cell decompositions of character varieties) [1](#)
- [2] Roger Casals, Eugene Gorsky, Mikhail Gorsky, José Simental. Algebraic weaves and braid varieties. *American Journal of Mathematics*, [arXiv:2012.06931](#). [1](#)
- [3] Roger Casals, Eugene Gorsky, Mikhail Gorsky, Ian Le, Linhui Shen, José Simental. Cluster structures on braid varieties. *Journal of the American Mathematical Society*, 2025. [arXiv:2207.11607](#). [1](#), [2.2](#)

## APPENDIX A. COMPUTATION

Firstly, we need to define the class of matrices over non-commutative rings which is not properly defined in SageMath.

```

class Matrix(list): # for any ring
    def __add__(self, other):
        res = [[self[i][j]+other[i][j] for j in range(len(other[0]))] for i in range(
len(self))]
        return Matrix(res)
    def __sub__(self, other):
        res = [[self[i][j]-other[i][j] for j in range(len(other[0]))] for i in range(
len(self))]
        return Matrix(res)
    def __mul__(self, other):
        if type(other)==Matrix:
            res = [[sum(self[i][k]*other[k][j] for k in range(len(self[0]))) for j in
range(len(other[0]))] for i in range(len(self))]
            return Matrix(res)
        else:
            return Matrix([[other*self[i][j] for j in range(len(self[0]))] for i in
range(len(self))])
    def __pow__(self, n):
        if n==0:
            return Matrix([[1 if i==j else 0] for j in range(len(self[0]))] for i in
range(len(self)))
        elif n== -1:
            res = matrix(self)^(-1)
            return Matrix([list(row) for row in res])
        elif n < -1:
            return (self^(-1))^( -n)
        else:
            return self^(n-1)*self
    def trace(self):
        return sum(self[i][i] for i in range(len(self)))
    def __repr__(self):
        res = ""
        width = [max(len(str(self[i][j])) for i in range(len(self))) for j in range(len(
self[0]))]
        for i in range(len(self)):
            row = " ".join(str(self[i][j]).rjust(width[j]) for j in range(len(self[0])
))
            res+= "["+row+"\n"
        return res[:-1]

def d(omega):
    if type(omega) == type(Diff.an_element()):
        mydict= omega.dict()
        def monomial(*arg):

```

```

        res = Diff(1)
        for i in range(len(Diff.gens())):
            if arg[i]==1:
                res = res*Diff.gens()[i]
        return res
    return sum(d(mydict[ind])*monomial(*ind) for ind in mydict)
if type(omega) == Matrix:
    return Matrix([[d(omega[i][j]) for j in range(len(omega[0]))] for i in range(
len(omega))])
elif "derivative" not in dir(omega):
    return 0
else:
    return sum(omega.derivative(Poly.gens()[i])*Diff.gens()[i] for i in range(len(
Poly.gens()))))
def thetaL(M):
    return M^(-1)*d(M)
def thetaR(M):
    return d(M)*M^(-1)
def beta(*ary):
    if len(ary)<=1: return 0
    if len(ary)==2: return (thetaL(ary[0])*thetaR(ary[1])).trace()
    newary = list(ary[:-2])+[ary[-2]*ary[-1]]
    return beta(*newary)+beta(ary[-2],ary[-1])
def Omega(M):
    return 1/3*(thetaL(M)^3).trace()

```

```

n = 2
x_names = ["x"+str(i)+str(j) for i in [1..n] for j in [1..n]]
x_names+= ["y"+str(i)+str(j) for i in [1..n] for j in [1..n]]
x_names+= ["z"+str(i)+str(j) for i in [1..n] for j in [1..n]]

d_names = ["d"+var for var in x_names]
Poly = PolynomialRing(QQ,x_names).fraction_field(); exec("\n".join("%s = Poly.gens()[%s
]"%(x_names[i],i) for i in range(len(x_names))))
Diff = GradedCommutativeAlgebra(Poly,d_names);

X = Matrix([[Poly.gens()[i*n+j] for j in range(n)]for i in range(n)])
Y = Matrix([[Poly.gens()[n^2+i*n+j] for j in range(n)]for i in range(n)])
Z = Matrix([[Poly.gens()[2*n^2+i*n+j] for j in range(n)]for i in range(n)])
print(thetaL(X))
print(beta(X,Y))
print(Omega(X) == 1/3*(thetaR(X)^3).trace())
print(d(beta(X,Y)) == Omega(X)+Omega(Y)-Omega(X*Y))
print(0 == beta(Y,Z)-beta(X*Y,Z)+beta(X,Y*Z)-beta(X,Y))

```



## APPENDIX B. EXPLICIT COMPUTATION

The figure shows four rows of braid diagrams, commutative diagrams, and formulas.

- Row 1:** A braid diagram with three strands labeled  $\tilde{z}_1, u_1$  (red),  $\tilde{z}_2, u_2$  (red), and  $\tilde{z}_3, u_3$  (red). A yellow arrow labeled  $\tilde{U}$  points from the bottom to the top. The commutative diagram is a square with horizontal arrows  $B_i(\tilde{z}_1, u_1)$  and  $B_i(\tilde{z}_2, u_2)$  on top, and  $B_i(\tilde{z}_3, u_3)$  on the bottom. A vertical arrow labeled  $\tilde{U}$  points from the bottom to the top. The formula is  $\omega - \omega' = -2 \frac{du_1 du_2}{u_1 u_2} + 2 \frac{du_1 du_3}{u_1 u_3} - 2 \frac{du_2 du_3}{u_2 u_3}$ .
- Row 2:** A braid diagram with three strands labeled  $\tilde{z}_1, u_1$  (red),  $\tilde{z}_2, u_2$  (red), and  $\tilde{z}'_1, u'_1$  (red). A yellow arrow labeled  $\tilde{U}$  points from the bottom to the top. The commutative diagram is a square with horizontal arrows  $B_i(\tilde{z}_1, u_1)$  and  $B_j(\tilde{z}_2, u_2)$  on top, and  $B_j(\tilde{z}'_1, u'_1)$  and  $B_i(\tilde{z}'_1, u'_1)$  on the bottom. The formula is  $\omega = \omega' = 0$ .
- Row 3:** A braid diagram with three strands labeled  $\tilde{z}_1, u_1$  (red),  $\tilde{z}_2, u_2$  (red), and  $\tilde{z}_3, u_3$  (red). A yellow arrow labeled  $\tilde{U}$  points from the bottom to the top. The commutative diagram is a square with horizontal arrows  $B_i(\tilde{z}_1, u_1)$ ,  $B_j(\tilde{z}_2, u_2)$ , and  $B_i(\tilde{z}_3, u_3)$  on top, and  $B_j(\tilde{z}'_1, u'_1)$ ,  $B_i(\tilde{z}'_2, u'_2)$ , and  $B_j(\tilde{z}'_3, u'_3)$  on the bottom. The formula is  $\omega = \frac{du_1 du_2}{u_1 u_2} - \frac{du_1 du_3}{u_1 u_3} + \frac{du_2 du_3}{u_2 u_3}$  and  $\omega' = \frac{du'_1 du'_2}{u'_1 u'_2} - \frac{du'_1 du'_3}{u'_1 u'_3} + \frac{du'_2 du'_3}{u'_2 u'_3}$ .
- Row 4:** A braid diagram with three strands labeled  $\tilde{z}, u$  (red),  $\tilde{z}', u'$  (red), and  $\tilde{z}, u$  (red). A yellow arrow labeled  $\tilde{U}$  points from the bottom to the top. The commutative diagram is a square with horizontal arrows  $B_i(\tilde{z}, u)$  on top and  $B_i(\tilde{z}', u')$  on the bottom. A vertical arrow labeled  $\tilde{U}$  points from the bottom to the top. The formula is  $\omega = \omega' = 0$ .

```
x_names = ["u1", "u2", "u3", "z3"]

d_names = ["d"+var for var in x_names]
Poly = PolynomialRing(QQ, x_names).fraction_field(); exec("\n".join("%s = Poly.gens()[%s]"
    ]%(x_names[i], i) for i in range(len(x_names))))
Diff = GradedCommutativeAlgebra(Poly, d_names);

z2 = u3/(u1*u2)
z1 = z3 + u2/(u1*u3)
a = -u1/(u2*u3)
B = lambda z,u: Matrix([[u*z, -u^(-1)], [u, 0]])
U = Matrix([[1, a], [0, 1]])
print(B(z1, u1)*B(z2, u2)==B(z3, u3)*U)
beta(B(z1, u1), B(z2, u2)) - beta(B(z3, u3), U)
```

True

$-2/(u1*u2)*du1*du2 + 2/(u1*u3)*du1*du3 - 2/(u2*u3)*du2*du3$

```
x_names = ["u1", "u2", "z1", "z2"]
```

```
d_names = ["d"+var for var in x_names]
```

```

Poly = PolynomialRing(QQ,x_names).fraction_field(); exec("\n".join("%s = Poly.gens()[%s
]"%(x_names[i],i) for i in range(len(x_names))))
Diff = GradedCommutativeAlgebra(Poly,d_names);

B1 = lambda z,u: Matrix([[u*z,-u^(-1),0,0],[u,0,0,0],[0,0,1,0],[0,0,0,1]])
B3 = lambda z,u: Matrix([[1,0,0,0],[0,1,0,0],[0,0,u*z,-u^(-1)],[0,0,u,0]])
beta(B1(z1,u1),B3(z2,u2))

```

0

```

x_names = ["u1","u2","u3","z1","z2","z3"]

d_names = ["d"+var for var in x_names]
Poly = PolynomialRing(QQ,x_names).fraction_field(); exec("\n".join("%s = Poly.gens()[%s
]"%(x_names[i],i) for i in range(len(x_names))))
Diff = GradedCommutativeAlgebra(Poly,d_names);

B1 = lambda z,u: Matrix([[u*z,-u^(-1),0],[u,0,0],[0,0,1]])
B2 = lambda z,u: Matrix([[1,0,0],[0,u*z,-u^(-1)],[0,u,0]])

beta(B1(z1,u1),B2(z2,u2),B1(z3,u3))

```

$$1/(u_1 u_2) du_1 du_2 - 1/(u_1 u_3) du_1 du_3 + 1/(u_2 u_3) du_2 du_3$$

```

x_names = ["u","z","zp","a"]

d_names = ["d"+var for var in x_names]
Poly = PolynomialRing(QQ,x_names).fraction_field(); exec("\n".join("%s = Poly.gens()[%s
]"%(x_names[i],i) for i in range(len(x_names))))
Diff = GradedCommutativeAlgebra(Poly,d_names);

ap = 0; up = u; a = -z+zp

B = lambda z,u: Matrix([[u*z,-u^(-1)],[u,0]])
U = Matrix([[1,a],[0,1]]); Up = Matrix([[1,ap],[0,1]])
print(U*B(z,u)==B(zp,up)*Up)
print(beta(U,B(z,u)))
print(beta(B(zp,up),Up))

```

True

0

0